Result.Loop.forIn.loop.partial_correctness3 coinflip experiment

proofs/Symcrust/Properties/While.lean
@@ -99,6 +99,20 @@ theorem Result.Loop.forIn.loop.partial_correctness2 {β : Type u} (f : Unit → 
   (Loop.forIn.loop f b = ok r ∨ Loop.forIn.loop f b = fail e) → motive b r e := by
   sorry
 
+theorem Result.Loop.forIn.loop.partial_correctness3 {β : Type u} (f : Unit → β → Result (ForInStep β))
+  (motive : β → Result β → Prop) :
+  (∀ (loop : β → Result β),
+    (∀ b : β, loop b ≠ div → motive b (loop b)) →
+      ∀ b : β, ∀ r : Result β, r ≠ div →
+        (do
+          let __do_lift ← f () b
+          match __do_lift with
+            | ForInStep.done b => pure b
+            | ForInStep.yield b => loop b) =
+        r → motive b r
+  ) → ∀ (b : β) (r : Result β), Loop.forIn.loop f b = r → motive b r := by
+  sorry
+
 @[progress]
 theorem Result.Loop.forIn.progress_spec {β : Type u} (l : Loop) (init : β)
   (f : Unit → β → Result (ForInStep β)) (hdiv : Result.Loop.forIn l init f ≠ div)
@@ -106,5 +120,46 @@ theorem Result.Loop.forIn.progress_spec {β : Type u} (l : Loop) (init : β)
   ∃ r, Result.Loop.forIn l init f = ok r ∧ Result.Loop.forIn l init f = ok r := by
   revert hdiv hfail
   cases (forIn l init f) <;> simp
+
+def whileLoop {β : Type u} (b : β) (f : β → Result (ForInStep β)) : Result β := do
+  match ← f b with
+    | ForInStep.done b  => pure b
+    | ForInStep.yield b => whileLoop b f
+partial_fixpoint
+
+theorem whileLoop.partial_correctness2 {β : Type u} (f : β → Result (ForInStep β))
+  (motive : β → β → Error → Prop) :
+  (∀ (loop : β → Result β),
+    (∀ b : β, ∀ r : β, ∀ e : Error, (loop b = ok r → motive b r e) ∧ (loop b = fail e → motive b r e)) →
+      ∀ b : β, ∀ r : β, ∀ e : Error,
+        ((do
+          let __do_lift ← f b
+          match __do_lift with
+            | ForInStep.done b => pure b
+            | ForInStep.yield b => loop b) =
+        ok r → motive b r e) ∧
+        ((do
+          let __do_lift ← f b
+          match __do_lift with
+            | ForInStep.done b => pure b
+            | ForInStep.yield b => loop b) =
+        fail e → motive b r e)
+  ) → ∀ (b r : β) (e : Error),
+  (whileLoop b f = ok r ∨ whileLoop b f = fail e) → motive b r e := by
+  sorry
+
+theorem whileLoop.partial_correctness3 {β : Type u} (f : β → Result (ForInStep β))
+  (motive : β → Result β → Prop) :
+  (∀ (loop : β → Result β),
+    (∀ b : β, loop b ≠ div → motive b (loop b)) →
+      ∀ b : β, ∀ r : Result β, r ≠ div →
+        (do
+          let __do_lift ← f b
+          match __do_lift with
+            | ForInStep.done b => pure b
+            | ForInStep.yield b => loop b) =
+        r → motive b r
+  ) → ∀ (b : β) (r : Result β), whileLoop b f = r → motive b r := by
+  sorry
 
 end CustomLoops
