proofs/Symcrust/Properties/Coinflip4.lean
@@ -56,8 +56,7 @@ theorem resFlipCoinThm (flip : Nat → Bool) :
       unfold loop_body at h3
       split at h3
       . next hb =>
-        rw [pure, instPureResult] at h3
-        simp only [bind_tc_ok] at h3
+        simp only [pure, bind_tc_ok] at h3
         have h5 := (hloop ⟨flip b.2, b.2 + 2⟩ r e).1 h3
         unfold motive at h5
         rw [CustomLoops.Result.Loop.forIn, CustomLoops.Result.Loop.forIn.loop] at h4
@@ -116,3 +115,75 @@ theorem resFlipCoinThm (flip : Nat → Bool) :
           apply (hloop ⟨flip b.2, b.2 + 2⟩ r3 e3).2 h3
           simp only [Nat.dvd_add_self_right, hb2]
         . simp [pure]
+
+set_option pp.showLetValues true in
+theorem resFlipCoinThm2 (flip : Nat → Bool) :
+  resFlipCoin flip ≠ div → ∃ i, resFlipCoin flip = ok i ∧ 2 ∣ i := by
+  intro hDiv
+  unfold resFlipCoin
+  simp only [Bool.not_eq_eq_eq_not, Bool.not_true]
+  tlet loop_body : Unit → MProd Bool ℕ → Result (ForInStep (MProd Bool ℕ)) :=
+    fun x r =>
+      if r.fst = false then do
+        pure PUnit.unit
+        pure (ForInStep.yield ⟨flip r.snd, r.snd + 2⟩)
+      else pure (ForInStep.done ⟨r.fst, r.snd⟩)
+  have : ∃ r' e', CustomLoops.Result.Loop.forIn.loop loop_body ⟨false, 0⟩ = ok r' ∨
+    CustomLoops.Result.Loop.forIn.loop loop_body ⟨false, 0⟩ = fail e' := by
+    rcases hDiv2 : CustomLoops.Result.Loop.forIn.loop loop_body ⟨false, 0⟩ with r' | e'
+    . apply Exists.intro r'
+      apply Exists.intro Error.panic -- Need this because `Error` doesn't have `deriving Inhabited`
+      simp
+    . apply Exists.intro ⟨false, 0⟩
+      apply Exists.intro e'
+      simp
+    . unfold resFlipCoin at hDiv
+      rw [forIn, CustomLoops.instForInResultLoopUnit_symcrust] at hDiv
+      simp at hDiv
+      rw [CustomLoops.Result.Loop.forIn, hDiv2] at hDiv
+      simp at hDiv
+  rcases this with ⟨r, e, h2⟩
+  let* ⟨r2, hr2⟩ ← CustomLoops.Result.Loop.forIn.progress_spec
+  . unfold resFlipCoin at hDiv
+    rw [forIn, CustomLoops.instForInResultLoopUnit_symcrust] at hDiv
+    simp only [Bool.not_eq_eq_eq_not, Bool.not_true, ne_eq] at hDiv
+    intro h2
+    rw [h2] at hDiv
+    simp at hDiv
+  . intro e2
+    rcases h2 with h2 | h2
+    . simp [CustomLoops.Result.Loop.forIn, h2]
+    . let motive : MProd Bool ℕ → Result (MProd Bool ℕ) → Prop := fun b _ =>
+        CustomLoops.Result.Loop.forIn Lean.Loop.mk b loop_body ≠ fail e2
+      apply CustomLoops.Result.Loop.forIn.loop.partial_correctness3 loop_body motive _ ⟨false, 0⟩ (fail e) h2
+      intro loop hloop b r3 hDiv2 h h3
+      unfold loop_body at h
+      split at h
+      . next hb =>
+        simp only [pure, bind_tc_ok] at h
+        specialize hloop ⟨flip b.2, b.2 + 2⟩
+        rw [h] at hloop
+        specialize hloop hDiv2
+        unfold motive at hloop
+        rw [CustomLoops.Result.Loop.forIn, CustomLoops.Result.Loop.forIn.loop] at h3
+        unfold loop_body at h3 hloop
+        simp only [hb, ↓reduceIte, pure, bind_tc_ok] at h3 hloop
+        rw [CustomLoops.Result.Loop.forIn] at hloop
+        exact hloop h3
+      . next hb =>
+        simp only [pure, hb, bind_tc_ok] at h
+        rw [CustomLoops.Result.Loop.forIn, CustomLoops.Result.Loop.forIn.loop] at h3
+        unfold loop_body at h3
+        simp [hb, pure] at h3
+  . rw [forIn, CustomLoops.instForInResultLoopUnit_symcrust]
+    simp only [hr2, bind_tc_ok, ok.injEq, exists_eq_left', loop_body]
+    let motive : MProd Bool ℕ → Result (MProd Bool ℕ) → Prop := fun b r => ∀ r', r = ok r' → 2 ∣ b.2 → 2 ∣ r'.2
+    have : 2 ∣ 0 := by omega
+    revert this
+    have test := CustomLoops.Result.Loop.forIn.loop.partial_correctness3 loop_body motive
+    unfold motive at test
+    -- Proof that coinFlip doesn't fail goes through a bit more easily for partial_correctness3, but,
+    -- expressing the motive for the actual case seems to be harder. As best as I can tell, there isn't actually
+    -- a motive I can write that will let me simply `apply` partial_correctness3 (I have to instantiate
+    -- partial_correctness3 and then use the result along with `hr2` to derive the goal)
+    sorry
