proofs/Symcrust/Properties/Temp.lean
@@ -1,0 +1,391 @@
+import Symcrust.Spec
+import Symcrust.Code.Funs
+import Symcrust.Properties.Basic
+
+#setup_aeneas_simps
+
+namespace Symcrust.ntt
+
+open Symcrust.Spec
+open Aeneas Aeneas.Std Aeneas.SRRange Result
+set_option linter.dupNamespace false
+set_option linter.hashCommand false
+set_option linter.unusedVariables false
+
+set_option maxHeartbeats 1000000
+
+open CustomLoops in
+def poly_element_sample_ntt_from_shake128_modified
+  (p_state : hash.HashState) (pe_dst : Array U16 256#usize) :
+  Result (hash.HashState × (Array U16 256#usize))
+  :=
+  do
+  let shake_output_buf := Array.repeat 24#usize 0#u8
+  let s ← (↑(Array.to_slice shake_output_buf) : Result (Slice U8))
+  let curr_buf_index := Slice.len s
+  -- Before while loop, instantiate mutable variables corresponding to arguments that would
+  -- have been created for the auxiliary recurisve function
+  let mut p_state := p_state
+  let mut pe_dst := pe_dst
+  let mut i := 0#usize
+  let mut shake_output_buf := shake_output_buf
+  let mut curr_buf_index := curr_buf_index
+  while i < key.MLWE_POLYNOMIAL_COEFFICIENTS do
+    let s ← (↑(Array.to_slice shake_output_buf) : Result (Slice U8))
+    let i1 := Slice.len s
+    massert (curr_buf_index <= i1)
+    let s1 ← (↑(Array.to_slice shake_output_buf) : Result (Slice U8))
+    let i2 := Slice.len s1
+    if curr_buf_index = i2
+    then
+      do
+      let (s2, to_slice_mut_back) ←
+        (↑(Array.to_slice_mut shake_output_buf) : Result ((Slice U8) ×
+          (Slice U8 → Array U8 24#usize)))
+      let (p_state1, s3) ← hash.shake128_extract p_state s2 false
+      let shake_output_buf1 := to_slice_mut_back s3
+      let s4 ← (↑(Array.to_slice shake_output_buf1) : Result (Slice U8))
+      let a ← ntt.slice_to_sub_array2 s4 0#usize
+      let i3 ← (↑(core.num.U16.from_le_bytes a) : Result U16)
+      let sample0 ← (↑(i3 &&& 4095#u16) : Result U16)
+      let s5 ← (↑(Array.to_slice shake_output_buf1) : Result (Slice U8))
+      let i4 ← 0#usize + 1#usize
+      let a1 ← ntt.slice_to_sub_array2 s5 i4
+      let i5 ← (↑(core.num.U16.from_le_bytes a1) : Result U16)
+      let sample1 ← i5 >>> 4#i32
+      let curr_buf_index1 ← 0#usize + 3#usize
+      let i6 ← (↑(UScalar.cast .U32 sample0) : Result U32)
+      let i7 ←
+        (↑(UScalar.cast_fromBool .Usize (i6 < ntt.Q)) : Result Usize)
+      let i8 ← i + i7
+      if i8 < key.MLWE_POLYNOMIAL_COEFFICIENTS
+      then
+        do
+        let pe_dst1 ← Array.update pe_dst i sample0
+        let pe_dst2 ← Array.update pe_dst1 i8 sample1
+        let i9 ← (↑(UScalar.cast .U32 sample1) : Result U32)
+        let i10 ←
+          (↑(UScalar.cast_fromBool .Usize (i9 < ntt.Q)) : Result Usize)
+        let i11 ← i8 + i10
+        -- Wherever the auxiliary recursive function would have terminated, instead set the mutable variables
+        -- with the values that would have been passed into the recursive call
+        p_state := p_state1
+        pe_dst := pe_dst2
+        i := i11
+        shake_output_buf := shake_output_buf1
+        curr_buf_index := curr_buf_index1
+      else
+        do
+        let pe_dst1 ← Array.update pe_dst i sample0
+        -- Wherever the auxiliary recursive function would have terminated, instead set the mutable variables
+        -- with the values that would have been passed into the recursive call
+        p_state := p_state1
+        pe_dst := pe_dst1
+        i := i8
+        shake_output_buf := shake_output_buf1
+        curr_buf_index := curr_buf_index1
+    else
+      do
+      let s2 ← (↑(Array.to_slice shake_output_buf) : Result (Slice U8))
+      let a ← ntt.slice_to_sub_array2 s2 curr_buf_index
+      let i3 ← (↑(core.num.U16.from_le_bytes a) : Result U16)
+      let sample0 ← (↑(i3 &&& 4095#u16) : Result U16)
+      let s3 ← (↑(Array.to_slice shake_output_buf) : Result (Slice U8))
+      let i4 ← curr_buf_index + 1#usize
+      let a1 ← ntt.slice_to_sub_array2 s3 i4
+      let i5 ← (↑(core.num.U16.from_le_bytes a1) : Result U16)
+      let sample1 ← i5 >>> 4#i32
+      let curr_buf_index1 ← curr_buf_index + 3#usize
+      let i6 ← (↑(UScalar.cast .U32 sample0) : Result U32)
+      let i7 ←
+        (↑(UScalar.cast_fromBool .Usize (i6 < ntt.Q)) : Result Usize)
+      let i8 ← i + i7
+      if i8 < key.MLWE_POLYNOMIAL_COEFFICIENTS
+      then
+        do
+        let pe_dst1 ← Array.update pe_dst i sample0
+        let pe_dst2 ← Array.update pe_dst1 i8 sample1
+        let i9 ← (↑(UScalar.cast .U32 sample1) : Result U32)
+        let i10 ←
+          (↑(UScalar.cast_fromBool .Usize (i9 < ntt.Q)) : Result Usize)
+        let i11 ← i8 + i10
+        -- Wherever the auxiliary recursive function would have terminated, instead set the mutable variables
+        -- with the values that would have been passed into the recursive call
+        p_state := p_state
+        pe_dst := pe_dst2
+        i := i11
+        shake_output_buf := shake_output_buf
+        curr_buf_index := curr_buf_index1
+      else
+        do
+        let pe_dst1 ← Array.update pe_dst i sample0
+        -- Wherever the auxiliary recursive function would have terminated, instead set the mutable variables
+        -- with the values that would have been passed into the recursive call
+        p_state := p_state
+        pe_dst := pe_dst1
+        i := i8
+        shake_output_buf := shake_output_buf
+        curr_buf_index := curr_buf_index1
+  ok (p_state, pe_dst)
+
+open CustomLoops in
+def poly_element_sample_ntt_from_shake128_modified2
+  (p_state : hash.HashState) (pe_dst : Array U16 256#usize) :
+  Result (hash.HashState × (Array U16 256#usize))
+  :=
+  do
+  let shake_output_buf := Array.repeat 24#usize 0#u8
+  let s ← (↑(Array.to_slice shake_output_buf) : Result (Slice U8))
+  let curr_buf_index := Slice.len s
+  let (p_state, pe_dst, i, shake_output_buf, curr_buf_index) ←
+    whileLoop (p_state, pe_dst, 0#usize, shake_output_buf, curr_buf_index) $
+    fun (p_state, pe_dst, i, shake_output_buf, curr_buf_index) => do
+      if i < key.MLWE_POLYNOMIAL_COEFFICIENTS
+      then
+        do
+        let s ← (↑(Array.to_slice shake_output_buf) : Result (Slice U8))
+        let i1 := Slice.len s
+        massert (curr_buf_index <= i1)
+        let s1 ← (↑(Array.to_slice shake_output_buf) : Result (Slice U8))
+        let i2 := Slice.len s1
+        if curr_buf_index = i2
+        then
+          do
+          let (s2, to_slice_mut_back) ←
+            (↑(Array.to_slice_mut shake_output_buf) : Result ((Slice U8) ×
+              (Slice U8 → Array U8 24#usize)))
+          let (p_state1, s3) ← hash.shake128_extract p_state s2 false
+          let shake_output_buf1 := to_slice_mut_back s3
+          let s4 ← (↑(Array.to_slice shake_output_buf1) : Result (Slice U8))
+          let a ← ntt.slice_to_sub_array2 s4 0#usize
+          let i3 ← (↑(core.num.U16.from_le_bytes a) : Result U16)
+          let sample0 ← (↑(i3 &&& 4095#u16) : Result U16)
+          let s5 ← (↑(Array.to_slice shake_output_buf1) : Result (Slice U8))
+          let i4 ← 0#usize + 1#usize
+          let a1 ← ntt.slice_to_sub_array2 s5 i4
+          let i5 ← (↑(core.num.U16.from_le_bytes a1) : Result U16)
+          let sample1 ← i5 >>> 4#i32
+          let curr_buf_index1 ← 0#usize + 3#usize
+          let i6 ← (↑(UScalar.cast .U32 sample0) : Result U32)
+          let i7 ←
+            (↑(UScalar.cast_fromBool .Usize (i6 < ntt.Q)) : Result Usize)
+          let i8 ← i + i7
+          if i8 < key.MLWE_POLYNOMIAL_COEFFICIENTS
+          then
+            do
+            let pe_dst1 ← Array.update pe_dst i sample0
+            let pe_dst2 ← Array.update pe_dst1 i8 sample1
+            let i9 ← (↑(UScalar.cast .U32 sample1) : Result U32)
+            let i10 ←
+              (↑(UScalar.cast_fromBool .Usize (i9 < ntt.Q)) : Result Usize)
+            let i11 ← i8 + i10
+            ForInStep.yield (p_state1, pe_dst2, i11, shake_output_buf1, curr_buf_index1)
+          else
+            do
+            let pe_dst1 ← Array.update pe_dst i sample0
+            ForInStep.yield (p_state1, pe_dst1, i8, shake_output_buf1, curr_buf_index1)
+        else
+          do
+          let s2 ← (↑(Array.to_slice shake_output_buf) : Result (Slice U8))
+          let a ← ntt.slice_to_sub_array2 s2 curr_buf_index
+          let i3 ← (↑(core.num.U16.from_le_bytes a) : Result U16)
+          let sample0 ← (↑(i3 &&& 4095#u16) : Result U16)
+          let s3 ← (↑(Array.to_slice shake_output_buf) : Result (Slice U8))
+          let i4 ← curr_buf_index + 1#usize
+          let a1 ← ntt.slice_to_sub_array2 s3 i4
+          let i5 ← (↑(core.num.U16.from_le_bytes a1) : Result U16)
+          let sample1 ← i5 >>> 4#i32
+          let curr_buf_index1 ← curr_buf_index + 3#usize
+          let i6 ← (↑(UScalar.cast .U32 sample0) : Result U32)
+          let i7 ←
+            (↑(UScalar.cast_fromBool .Usize (i6 < ntt.Q)) : Result Usize)
+          let i8 ← i + i7
+          if i8 < key.MLWE_POLYNOMIAL_COEFFICIENTS
+          then
+            do
+            let pe_dst1 ← Array.update pe_dst i sample0
+            let pe_dst2 ← Array.update pe_dst1 i8 sample1
+            let i9 ← (↑(UScalar.cast .U32 sample1) : Result U32)
+            let i10 ←
+              (↑(UScalar.cast_fromBool .Usize (i9 < ntt.Q)) : Result Usize)
+            let i11 ← i8 + i10
+            ForInStep.yield (p_state, pe_dst2, i11, shake_output_buf, curr_buf_index1)
+          else
+            do
+            let pe_dst1 ← Array.update pe_dst i sample0
+            ForInStep.yield (p_state, pe_dst1, i8, shake_output_buf, curr_buf_index1)
+      else ForInStep.done (p_state, pe_dst, i, shake_output_buf, curr_buf_index)
+  ok (p_state, pe_dst)
+
+/- This is not the infinite stream axiomatization that we discussed, but it is a consequence that follows
+   from it. Tentatively, I believe this is the only fact required for
+   `poly_element_sample_ntt_from_shake128_modified`, but if I am incorrect, this axiom can be replaced with
+   a theorem that derives this fact from the infinite stream axiomatization. -/
+axiom XOF.squeeze.composable (ctx : SHAKE128.Context) (z1 z2 : Nat) :
+  let (ctx'_part1, v1) := XOF.squeeze ctx z1
+  let (ctx'_part2, v2) := XOF.squeeze ctx'_part1 z2
+  let (ctx', v) := XOF.squeeze ctx (z1 + z2)
+  ctx'_part2 = ctx' ∧ v1 ++ v2 = v
+
+-- **TODO** It might instead be better to have the reverse mapping, not sure
+axiom SHAKE128.Context.ofHashState (s : hash.HashState) : SHAKE128.Context
+
+axiom shake128_extract.length_inv :
+  ∀ s l r, hash.shake128_extract s l false = ok r → r.2.1.length = l.length
+
+axiom SHAKE128.squeeze_eq_extract (s : hash.HashState) (n : ℕ) :
+  -- Second arg to shake128_extract is irrelevant (it is location of Rust output)
+  ∀ l, ∀ hl : l.length = n, ∃ r, ∃ h : hash.shake128_extract s l false = ok r,
+  XOF.squeeze (SHAKE128.Context.ofHashState s) n =
+  (SHAKE128.Context.ofHashState r.1,
+    ⟨(r.2.1.map U8.bv).toArray, by simp [shake128_extract.length_inv _ _ _ h, hl]⟩)
+
+set_option pp.analyze true in
+set_option pp.coercions.types true in
+set_option pp.analyze.typeAscriptions true in
+@[progress]
+def poly_element_sample_ntt_from_shake128_modified.spec (p_state : hash.HashState)
+  (pe_dst : Array U16 256#usize) (B : {l : List Byte // l.length = 34 })
+  (hB : XOF.absorb XOF.init B = SHAKE128.Context.ofHashState p_state)
+  (hDiv : poly_element_sample_ntt_from_shake128_modified p_state pe_dst ≠ div) :
+  ∃ r, poly_element_sample_ntt_from_shake128_modified p_state pe_dst = ok r ∧
+  sampleNTT B = some (to_poly r.2) := by
+  unfold poly_element_sample_ntt_from_shake128_modified
+  simp only [CustomLoops.instForInResultLoopUnit_symcrust, UScalar.lt_equiv,
+    key.MLWE_POLYNOMIAL_COEFFICIENTS_eq, UScalar.le_equiv, Usize.ofNat_val_eq, Q.eq,
+    UScalar.ofNat_val_eq, forIn, Spec.Q, Prod.exists]
+  let* ⟨s, hs⟩ ← Array.to_slice.progress_spec
+  let loop_state_type := MProd Usize
+    (MProd (UScalar UScalarTy.Usize)
+    (MProd hash.HashState (MProd (Std.Array U16 256#usize) (Std.Array (UScalar UScalarTy.U8) 24#usize))))
+  -- Automation note: It might be worthwhile to write a tactic that makes it simpler to extract the inner
+  -- loop body without having to painstakingly copy the loop body into a `tlet`
+  olet hloop_body : (loop_body : Unit → loop_state_type → Result (ForInStep loop_state_type)) :=
+    fun x (r : loop_state_type) =>
+      if (↑r.snd.fst : ℕ) < 256 then do
+        let s ← (↑r.snd.snd.snd.snd.to_slice : Result (Slice (UScalar UScalarTy.U8)))
+        massert ((↑r.fst : ℕ) ≤ (↑s : List (UScalar UScalarTy.U8)).length)
+        let s1 ← (↑r.snd.snd.snd.snd.to_slice : Result (Slice (UScalar UScalarTy.U8)))
+        if r.fst = s1.len then do
+            let __discr ←
+              (↑r.snd.snd.snd.snd.to_slice_mut :
+                  Result
+                    (Slice (UScalar UScalarTy.U8) ×
+                      (Slice (UScalar UScalarTy.U8) → Std.Array (UScalar UScalarTy.U8) 24#usize)))
+            let __discr_1 ← hash.shake128_extract r.snd.snd.fst __discr.1 false
+            let s4 ← (↑(__discr.2 __discr_1.2).to_slice : Result (Slice (UScalar UScalarTy.U8)))
+            let a ← slice_to_sub_array2 s4 0#usize
+            let i3 ← (↑(core.num.U16.from_le_bytes a) : Result U16)
+            let sample0 ← (↑(i3 &&& 4095#u16) : Result (UScalar UScalarTy.U16))
+            let s5 ← (↑(__discr.2 __discr_1.2).to_slice : Result (Slice (UScalar UScalarTy.U8)))
+            let i4 ← 0#usize + 1#usize
+            let a1 ← slice_to_sub_array2 s5 i4
+            let i5 ← (↑(core.num.U16.from_le_bytes a1) : Result U16)
+            let sample1 ← i5 >>> 4#i32
+            let curr_buf_index1 ← 0#usize + 3#usize
+            let i6 ← (↑(UScalar.cast UScalarTy.U32 sample0) : Result (UScalar UScalarTy.U32))
+            let i7 ←
+              (↑(UScalar.cast_fromBool UScalarTy.Usize (decide ((↑i6 : ℕ) < 3329))) :
+                  Result (UScalar UScalarTy.Usize))
+            let i8 ← r.snd.fst + i7
+            if (↑i8 : ℕ) < 256 then do
+                let pe_dst1 ← r.snd.snd.snd.fst.update r.snd.fst sample0
+                let pe_dst2 ← pe_dst1.update i8 sample1
+                let i9 ← (↑(UScalar.cast UScalarTy.U32 sample1) : Result (UScalar UScalarTy.U32))
+                let i10 ←
+                  (↑(UScalar.cast_fromBool UScalarTy.Usize (decide ((↑i9 : ℕ) < 3329))) :
+                      Result (UScalar UScalarTy.Usize))
+                let i11 ← i8 + i10
+                ok (ForInStep.yield ⟨curr_buf_index1, i11, __discr_1.1, pe_dst2, __discr.2 __discr_1.2⟩)
+              else do
+                let pe_dst1 ← r.snd.snd.snd.fst.update r.snd.fst sample0
+                ok (ForInStep.yield ⟨curr_buf_index1, i8, __discr_1.1, pe_dst1, __discr.2 __discr_1.2⟩)
+          else do
+            let s2 ← (↑r.snd.snd.snd.snd.to_slice : Result (Slice (UScalar UScalarTy.U8)))
+            let a ← slice_to_sub_array2 s2 r.fst
+            let i3 ← (↑(core.num.U16.from_le_bytes a) : Result U16)
+            let sample0 ← (↑(i3 &&& 4095#u16) : Result (UScalar UScalarTy.U16))
+            let s3 ← (↑r.snd.snd.snd.snd.to_slice : Result (Slice (UScalar UScalarTy.U8)))
+            let i4 ← r.fst + 1#usize
+            let a1 ← slice_to_sub_array2 s3 i4
+            let i5 ← (↑(core.num.U16.from_le_bytes a1) : Result U16)
+            let sample1 ← i5 >>> 4#i32
+            let curr_buf_index1 ← r.fst + 3#usize
+            let i6 ← (↑(UScalar.cast UScalarTy.U32 sample0) : Result (UScalar UScalarTy.U32))
+            let i7 ←
+              (↑(UScalar.cast_fromBool UScalarTy.Usize (decide ((↑i6 : ℕ) < 3329))) :
+                  Result (UScalar UScalarTy.Usize))
+            let i8 ← r.snd.fst + i7
+            if (↑i8 : ℕ) < 256 then do
+                let pe_dst1 ← r.snd.snd.snd.fst.update r.snd.fst sample0
+                let pe_dst2 ← pe_dst1.update i8 sample1
+                let i9 ← (↑(UScalar.cast UScalarTy.U32 sample1) : Result (UScalar UScalarTy.U32))
+                let i10 ←
+                  (↑(UScalar.cast_fromBool UScalarTy.Usize (decide ((↑i9 : ℕ) < 3329))) :
+                      Result (UScalar UScalarTy.Usize))
+                let i11 ← i8 + i10
+                ok (ForInStep.yield ⟨curr_buf_index1, i11, r.snd.snd.fst, pe_dst2, r.snd.snd.snd.snd⟩)
+              else do
+                let pe_dst1 ← r.snd.snd.snd.fst.update r.snd.fst sample0
+                ok (ForInStep.yield ⟨curr_buf_index1, i8, r.snd.snd.fst, pe_dst1, r.snd.snd.snd.snd⟩)
+      else ok (ForInStep.done ⟨r.fst, r.snd.fst, r.snd.snd.fst, r.snd.snd.snd.fst, r.snd.snd.snd.snd⟩)
+  let* ⟨r, hr⟩ ← CustomLoops.Result.Loop.forIn.progress_spec
+  . intro h
+    contrapose hDiv -- **TODO** Is there a better way to do this?
+    unfold poly_element_sample_ntt_from_shake128_modified
+    simp only [CustomLoops.instForInResultLoopUnit_symcrust, UScalar.lt_equiv,
+      key.MLWE_POLYNOMIAL_COEFFICIENTS_eq, UScalar.le_equiv, Usize.ofNat_val_eq, Q.eq,
+      UScalar.ofNat_val_eq, forIn, ne_eq, not_not]
+    let* ⟨s', hs'⟩ ← Array.to_slice.progress_spec
+    rw [hs] at h
+    rw [hs', ← hloop_body, h]
+    simp
+  . intro e
+    -- **PLAN** Use `cases poly_element_sample_ntt_from_shake128_modified p_state pe_dst`
+    -- to get the values for the second and third goals generated by
+    -- CustomLoops.Result.Loop.forIn.loop.partial_correctness2
+    let motive : loop_state_type → loop_state_type → Error → Prop := fun b _ _ =>
+      CustomLoops.Result.Loop.forIn Lean.Loop.mk b loop_body ≠ fail e
+    -- have test1 := CustomLoops.Result.Loop.forIn.loop.partial_correctness loop_body motive
+    -- have test2 := CustomLoops.Result.Loop.forIn.loop.partial_correctness2 loop_body motive
+    apply CustomLoops.Result.Loop.forIn.loop.partial_correctness2 loop_body motive
+      _ ⟨s.len, 0#usize, p_state, pe_dst, Array.repeat 24#usize 0#u8⟩
+    . sorry
+    . sorry
+    . sorry
+    . sorry
+  . sorry
+
+set_option pp.analyze true in
+set_option pp.coercions.types true in
+set_option pp.analyze.typeAscriptions true in
+@[progress]
+def poly_element_sample_ntt_from_shake128_modified2.spec (p_state : hash.HashState)
+  (pe_dst : Array U16 256#usize) (B : {l : List Byte // l.length = 34 })
+  (hB : XOF.absorb XOF.init B = SHAKE128.Context.ofHashState p_state)
+  (hDiv : poly_element_sample_ntt_from_shake128_modified p_state pe_dst ≠ div) :
+  ∃ r, poly_element_sample_ntt_from_shake128_modified2 p_state pe_dst = ok r ∧
+  sampleNTT B = some (to_poly r.2) := by
+  unfold poly_element_sample_ntt_from_shake128_modified2
+  simp only [CustomLoops.instForInResultLoopUnit_symcrust, UScalar.lt_equiv,
+    key.MLWE_POLYNOMIAL_COEFFICIENTS_eq, UScalar.le_equiv, Usize.ofNat_val_eq, Q.eq,
+    UScalar.ofNat_val_eq, forIn, Spec.Q, Prod.exists]
+  -- **NOTE** As soon as `simp` is called, the state used by `whileLoop` reverts to projections
+  -- rather than named matching
+  sorry
+
+structure myTest where
+  a : Nat
+  b : Nat
+
+def hi : myTest := {a := 2, b := 3}
+
+def getB (x : myTest) :=
+  match x with
+  | ⟨_, b⟩ => b
+
+def get2 (x : myTest) := x.2
+
+theorem test : getB hi = get2 hi := by
+  simp [getB]
+  sorry
